theories/AccInv.v
@@ -1,0 +1,55 @@
+
+
+(* this file justifies why we can suppose an object term acc_inv with the appropriate typing rule. 
+  indeed, by translating this proof into the object language, we would obtain implementations of the axioms 
+    Axiom accinv : level -> term -> term -> term -> term -> term -> term -> term.
+    Axiom type_accinv :
+        ∀ Γ i A R a p b r,
+        Γ ⊢< Ax i > A : Sort i ->
+        Γ ,, (i, A) ,, (i, A<[shift>>var]) ⊢< Ax prop > R : Sort prop -> 
+        Γ ⊢< i > a : A -> 
+        Γ ⊢< prop > p : acc i A R a -> 
+        Γ ⊢< i > b : A -> 
+        Γ ⊢< prop > r : R <[a.:b..] -> 
+        Γ ⊢< prop > accinv i A R a p b r : acc i A R b.  
+  *)
+
+Axiom Acc : forall (A : Type) (R : A -> A -> Prop) (a : A), Prop.
+
+Axiom acc_in : forall A R a, (forall y, R a y -> Acc A R y) -> Acc A R a.
+
+Axiom Acc_pre_ind : forall A R (P : A -> Prop) (p : forall a : A, (forall y : A, R a y -> P y) -> P a) (y : A) (r : Acc A R y), P y.
+
+Definition prod_prop (A B : Prop) : Prop := forall P, (A -> B -> P) -> P.
+
+Definition fst_prop {A B}: prod_prop A B -> A := fun f => f A (fun a b => a).
+
+Definition snd_prop {A B}: prod_prop A B -> B := fun f => f B (fun a b => b).
+
+Definition mk_prod_prop {A B} : A -> B -> prod_prop A B := fun a b P f => f a b.
+
+Lemma Acc_ind A R (P : A -> Prop) (p : forall a : A, (forall y, R a y -> Acc A R y) -> (forall y, R a y -> P y) -> P a) (y : A) (r : Acc A R y) : P y.
+Proof.
+  intros.
+  eapply snd_prop.
+  eapply (Acc_pre_ind _ _ (fun a => prod_prop (Acc A R a) (P a))).
+  2:exact r.
+  intros. eapply mk_prod_prop.
+  - eapply acc_in. intros. eapply H in H0. eapply (fst_prop H0).
+  - eapply p.
+    + intros. eapply H in H0.  eapply (fst_prop H0).
+    + intros. eapply H in H0. eapply (snd_prop H0). 
+Defined.
+
+Lemma acc_inv A R a : Acc A R a -> forall b, R a b -> Acc A R b.
+Proof.
+  intros.
+  eapply (Acc_ind _ _ (fun a => R a b -> Acc A R b)). 3:exact H0. 2:exact H.
+  intros. eapply H1. exact H3.
+Defined.
+
+(* the implementation of accinv would require us to write the term printed by the 
+  following command in the syntax specified in AST.v, and then retype it using 
+  the rules of Typing.v. by the above proofs, this would be theoretically possible
+  but practically infeasible, justifying why supposing these axioms is reasonable *)
+Eval cbv in acc_inv.
