theories/Typing.v
@@ -41,6 +41,10 @@ Reserved Notation "Γ ⊢< l > t : T" (at level 50, l, t, T at next level).
 Reserved Notation "Γ ⊢< l > t ≡ u : T" (at level 50, l, t, u, T at next level).
 Reserved Notation "⊢ Γ" (at level 50).
 
+
+(* see AccInv.v for a justification of this axiom *)
+Axiom accinv : level -> term -> term -> term -> term -> term -> term -> term.
+
 Inductive typing : ctx -> level -> term → term → Prop :=
 
 | type_var :
@@ -98,7 +102,37 @@ Inductive typing : ctx -> level -> term → term → Prop :=
       Γ ,, (ty 0 , Nat) ,, (l , P) ⊢< l > p_succ : P <[ (succ (var 1)) .: (shift >> (shift >> var)) ] ->
       Γ ⊢< ty 0 > t : Nat ->
       Γ ⊢< l > rec l P p_zero p_succ t : P <[ t .. ]
+
+| type_acc : 
+    ∀ Γ i A R a,
+    Γ ⊢< Ax i > A : Sort i ->
+    Γ ,, (i, A) ,, (i, S ⋅ A) ⊢< Ax prop > R : Sort prop -> 
+    Γ ⊢< i > a : A -> 
+    Γ ⊢< prop > acc i A R a : Sort prop
+
+| type_accin : 
+    ∀ Γ i A R a p,
+    Γ ⊢< Ax i > A : Sort i ->
+    Γ ,, (i, A) ,, (i, S ⋅ A) ⊢< Ax prop > R : Sort prop -> 
+    Γ ⊢< i > a : A -> 
+    let A_wk := (plus 2) ⋅ A in
+    let R_wk := (up_ren (up_ren (plus 2))) ⋅ R in
+    let acc_wk := acc i A_wk R_wk (var 1)  in
+    let R' := R <[(S ⋅ a) ..] in
+    Γ ⊢< prop > p : Pi i prop A (Pi prop prop R' acc_wk) ->
+    Γ ⊢< prop > accin i A R a p : acc i A R a
   
+| type_accel : 
+    ∀ Γ i l A R a q P p,
+    Γ ⊢< Ax i > A : Sort i ->
+    Γ ,, (i, A) ,, (i, S ⋅ A) ⊢< Ax prop > R : Sort prop -> 
+    Γ ,, (i, A) ⊢< Ax l > P : Sort l ->
+    let B := Pi i l (S ⋅ A) (Pi prop l R (S ⋅ (up_ren S) ⋅ P)) in
+    Γ ,, (i, A) ,, (Ru i l, B) ⊢< l > p : S ⋅ P ->
+    Γ ⊢< i > a : A -> 
+    Γ ⊢< prop > q : acc i A R a -> 
+    Γ ⊢< l > accel i l A R P p a q : P <[a ..]
+
 | type_conv : 
     ∀ Γ l A B t,
       Γ ⊢< l > t : A -> 
@@ -172,6 +206,37 @@ with conversion : ctx -> level -> term -> term -> term -> Prop :=
       Γ ,, (ty 0 , Nat) ,, (l , P) ⊢< l > p_succ ≡ p_succ' : P <[ (succ (var 1)) .: (shift >> (shift >> var)) ] ->
       Γ ⊢< ty 0 > t ≡ t' : Nat ->
       Γ ⊢< l > rec l P p_zero p_succ t ≡ rec l P' p_zero' p_succ' t' : P <[ t .. ]
+
+
+| conv_acc : 
+    ∀ Γ i A A' R R' a a',
+    Γ ⊢< Ax i > A ≡ A' : Sort i ->
+    Γ ,, (i, A) ,, (i, S ⋅ A) ⊢< Ax prop > R ≡ R' : Sort prop -> 
+    Γ ⊢< i > a ≡ a' : A -> 
+    Γ ⊢< prop > acc i A R a ≡ acc i A' R' a' : Sort prop
+
+| conv_accin : 
+    ∀ Γ i A A' R R' a a' p p',
+    Γ ⊢< Ax i > A ≡ A' : Sort i ->
+    Γ ,, (i, A) ,, (i, S ⋅ A) ⊢< Ax prop > R ≡ R' : Sort prop -> 
+    Γ ⊢< i > a ≡ a' : A -> 
+    let A_wk := (plus 2) ⋅ A in
+    let R_wk := (up_ren (up_ren (plus 2))) ⋅ R in
+    let acc_wk := acc i A_wk R_wk (var 1)  in
+    let R' := R <[(S ⋅ a) ..] in
+    Γ ⊢< prop > p ≡ p' : Pi i prop A (Pi prop prop R' acc_wk) ->
+    Γ ⊢< prop > accin i A R a p ≡ accin i A' R' a' p' : acc i A R a
+  
+| conv_accel : 
+    ∀ Γ i l A A' R R' a a' q q' P P' p p',
+    Γ ⊢< Ax i > A ≡ A' : Sort i ->
+    Γ ,, (i, A) ,, (i, S ⋅ A) ⊢< Ax prop > R ≡ R' : Sort prop -> 
+    Γ ,, (i, A) ⊢< Ax l > P ≡ P' : Sort l ->
+    let B := Pi i l (S ⋅ A) (Pi prop l R (S ⋅ (up_ren S) ⋅ P)) in
+    Γ ,, (i, A) ,, (Ru i l, B) ⊢< l > p ≡ p' : S ⋅ P ->
+    Γ ⊢< i > a ≡ a': A -> 
+    Γ ⊢< prop > q ≡ q' : acc i A R a -> 
+    Γ ⊢< l > accel i l A R P p a q ≡ accel i l A' R' P' p' a' q' : P <[a ..]
   
 | conv_conv : 
     ∀ Γ l A B t t',
@@ -219,6 +284,50 @@ with conversion : ctx -> level -> term -> term -> term -> Prop :=
       Γ ⊢< l > rec l P p_zero p_succ (succ t) ≡ 
           p_succ <[(rec l P p_zero p_succ t) .: t ..] : P <[ (succ t) .. ]
 
+| conv_accel_accin : 
+    ∀ Γ i l A R a q P p,
+    Γ ⊢< Ax i > A : Sort i ->
+    Γ ,, (i, A) ,, (i, S ⋅ A) ⊢< Ax prop > R : Sort prop -> 
+    Γ ,, (i, A) ⊢< Ax l > P : Sort l ->
+    let B := Pi i l (S ⋅ A) (Pi prop l R (S ⋅ (up_ren S) ⋅ P)) in
+    Γ ,, (i, A) ,, (Ru i l, B) ⊢< l > p : S ⋅ P ->
+    Γ ⊢< i > a : A -> 
+    Γ ⊢< prop > q : acc i A R a -> 
+    let t0 := accinv i ((plus 2) ⋅ A) ((up_ren (up_ren (plus 2))) ⋅ R) ((plus 2) ⋅ a) ((plus 2) ⋅ q) (var 1) (var 0) in
+    let t1 := accel i l A R P p (var 1) t0 in 
+    let t2 := R<[S ⋅ a .: (var 0 .: S >> var)] in 
+    let t3 := lam prop l t2 (S ⋅ P) t1 in
+    let t4 := Pi prop prop t2 (S ⋅ P) in
+    let t5 := lam i l A t4 t3 in
+    Γ ⊢< l > accel i l A R P p a q ≡ p <[ t5 .: a ..] : P <[a ..]
+(* 
+| conv_accel_accin : 
+    ∀ Γ i l A R a q P p,
+    Γ ⊢< Ax i > A : Sort i ->
+    Γ ,, (i, A) ,, (i, S ⋅ A) ⊢< Ax prop > R : Sort prop -> 
+    Γ ,, (i, A) ⊢< Ax l > P : Sort l ->
+    let B := Pi i l (S ⋅ A) (Pi prop l R (S ⋅ (up_ren S) ⋅ P)) in
+    Γ ,, (i, A) ,, (Ru i l, B) ⊢< l > p : S ⋅ P ->
+    Γ ⊢< i > a : A -> 
+    let A_wk := (plus 2) ⋅ A in
+    let R_wk := (up_ren (up_ren (plus 2))) ⋅ R in
+    let acc_wk := acc i A_wk R_wk (var 1)  in
+    let R' := R <[(S ⋅ a) ..] in
+    Γ ⊢< prop > q : Pi i prop A (Pi prop prop R' acc_wk) ->
+
+    let t1 := R<[(plus 3) ⋅ a .: (var 0 .: (plus 3) >> var)] in 
+    let t2 := acc i ((plus 4) ⋅ A) ((up_ren (up_ren (plus 4))) ⋅ R) (var 1) in
+    let t3 := app i prop ((plus 2) ⋅ A) (Pi prop prop t1 t2) ((plus 2) ⋅ q) (var 1) in
+    let t4 := R<[(plus 2) ⋅ a .: (var 1 .: (plus 2) >> var)] in 
+    let t5 := acc i ((plus 3) ⋅ A) ((up_ren (up_ren (plus 3))) ⋅ R) (var 2) in
+    let t6 := app prop prop t4 t5 t3 (var 0) in
+    let t7 := accel i l A R P p (var 1) t6 in 
+    let t8 := R<[S ⋅ a .: (var 0 .: S >> var)] in 
+    let t9 := lam prop l t8 (S ⋅ P) t7 in
+    let t10 := Pi prop prop t8 (S ⋅ P) in
+    let t11 := lam i l A t10 t9 in
+    Γ ⊢< l > accel i l A R P p a (accin i A R a q) ≡ p <[ t11 .: a ..] : P <[a ..] *)
+
 | conv_sym : 
     ∀ Γ l t u A,
       Γ ⊢< l > t ≡ u : A ->
@@ -234,11 +343,21 @@ where "Γ ⊢< l > t : A" := (typing Γ l t A)
 and   "⊢ Γ" := (ctx_typing Γ)
 and   "Γ ⊢< l > t ≡ u : A" := (conversion Γ l t u A).
 
-
 Scheme typing_mut := Induction for typing Sort Prop
 with conversion_mut := Induction for conversion Sort Prop.
 Combined Scheme typing_conversion_mutind from typing_mut, conversion_mut.
 
+
+(* see AccInv.v for a justification of this axiom *)
+Axiom type_accinv :
+    ∀ Γ i A R a p b r,
+    Γ ⊢< Ax i > A : Sort i ->
+    Γ ,, (i, A) ,, (i, A<[shift>>var]) ⊢< Ax prop > R : Sort prop -> 
+    Γ ⊢< i > a : A -> 
+    Γ ⊢< prop > p : acc i A R a -> 
+    Γ ⊢< i > b : A -> 
+    Γ ⊢< prop > r : R <[a.:b..] -> 
+    Γ ⊢< prop > accinv i A R a p b r : acc i A R b.
 
 Reserved Notation "Γ ⊢s σ : Δ" (at level 50, σ, Δ at next level).
 
